problem summary

theories/FOL/FOL.v
@@ -1,6 +1,6 @@
 (** * First-Order Logic *)
 
-From Undecidability.FOL.Util Require Import FOL_facts Deduction Semantics Kripke.
+From Undecidability.FOL.Util Require Import Syntax Deduction Tarski Kripke.
  
 (** ** Syntax as defined in Util/FOL_facts.v 
 
@@ -19,10 +19,20 @@ Inductive form : logic -> Type :=
 | All {b} : var -> form b -> form b.
 *)
 
-Notation "FOL*_prv_intu" := (@prv intu frag nil).
-Notation "FOL*_valid" := (@valid frag).
-Definition FOL_satis := @satis full.
-Definition FOL_valid_intu := (@kvalid full).
-Definition FOL_prv_intu := @prv intu full nil.
-Definition FOL_prv_class := @prv class full nil.
-Definition FOL_satis_intu := @ksatis full.
+Inductive syms_func := t_f : bool -> syms_func | t_e.
+
+Instance sig_func : funcs_signature :=
+  {| syms := syms_func; ar_syms := fun f => if f then 1 else 0 |}.
+
+Inductive syms_pred := Pr | Q.
+
+Instance sig_pred : preds_signature :=
+  {| preds := syms_pred; ar_preds := fun P => if P then 2 else 0 |}.
+
+Notation "FOL*_prv_intu" := (@prv _ _ falsity_off intu nil).
+Notation "FOL*_valid" := (@valid _ _ falsity_off).
+Definition FOL_satis := @satis _ _ falsity_on.
+Definition FOL_valid_intu := @kvalid _ _ falsity_on.
+Definition FOL_prv_intu := @prv _ _ falsity_on intu nil.
+Definition FOL_prv_class := @prv _ _ falsity_on class nil.
+Definition FOL_satis_intu := @ksatis _ _ falsity_on.
