theories/FOL/Util/Kripke.v
@@ -24,10 +24,9 @@ Section Kripke.
 
         k_interp : interp domain ;
         k_P : nodes -> forall P : preds, Vector.t domain (ar_preds P) -> Prop ;
-        k_Bot : nodes -> Prop ;
+        (* k_Bot : nodes -> Prop ; *)
 
         mon_P : forall u v, reachable u v -> forall P (t : Vector.t domain (ar_preds P)), k_P u t -> k_P v t;
-        mon_Bot : forall u v, reachable u v -> k_Bot u -> k_Bot v
       }.
 
     Variable M : kmodel.
@@ -35,19 +34,16 @@ Section Kripke.
     Fixpoint ksat {ff : falsity_flag} u (rho : nat -> domain) (phi : form) : Prop :=
       match phi with
       | atom P v => k_P u (Vector.map (@eval _ _ _ k_interp rho) v)
-      | falsity => k_Bot u
+      | falsity => False
       | bin Impl phi psi => forall v, reachable u v -> ksat v rho phi -> ksat v rho psi
       | quant All phi => forall j : domain, ksat u (j .: rho) phi
       end.
-
-    (*Global Instance kmodel_reach_refl : Reflexive reachable := reach_refl.
-    Global Instance kmodel_reach_trans : Transitive reachable := reach_tran.*)
 
     Lemma ksat_mon {ff : falsity_flag} (u : nodes) (rho : nat -> domain) (phi : form) :
       forall v (H : reachable u v), ksat u rho phi -> ksat v rho phi.
     Proof.
       revert rho.
-      induction phi; intros rho v' H; cbn; try destruct b0; try destruct q; intuition; eauto using mon_P, mon_Bot, reach_tran.
+      induction phi; intros rho v' H; cbn; try destruct b0; try destruct q; intuition; eauto using mon_P, reach_tran.
     Qed.
 
     Lemma ksat_iff {ff : falsity_flag} u rho phi :
@@ -59,18 +55,19 @@ Section Kripke.
     Qed.
   End Model.
 
-  Notation "rho  '⊨(' u ')'  phi" := (ksat _ u rho phi) (at level 20).
-  Notation "rho '⊨(' u , M ')' phi" := (@ksat _ M _ u rho phi) (at level 20).
+  Notation "rho  '⊩(' u ')'  phi" := (ksat _ u rho phi) (at level 20).
+  Notation "rho '⊩(' u , M ')' phi" := (@ksat _ M _ u rho phi) (at level 20).
   Arguments ksat {_ _ _} _ _ _, _ _ _ _ _ _.
 
-  Hint Resolve reach_refl.
+  Hint Resolve reach_refl : core.
 
   Section Substs.
+
     Variable D : Type.
     Context {M : kmodel D}.
 
     Lemma ksat_ext {ff : falsity_flag} u rho xi phi :
-      (forall x, rho x = xi x) -> rho ⊨(u,M) phi <-> xi ⊨(u,M) phi.
+      (forall x, rho x = xi x) -> rho ⊩(u,M) phi <-> xi ⊩(u,M) phi.
     Proof.
       induction phi in rho, xi, u |-*; intros Hext; comp.
       - tauto.
@@ -80,7 +77,7 @@ Section Kripke.
     Qed.
 
     Lemma ksat_comp {ff : falsity_flag} u rho xi phi :
-      rho ⊨(u,M) (subst_form xi phi) <-> (xi >> eval rho (I := @k_interp _ M)) ⊨(u,M) phi.
+      rho ⊩(u,M) phi[xi] <-> (xi >> eval rho (I := @k_interp _ M)) ⊩(u,M) phi.
     Proof.
       induction phi in rho, xi, u |-*; comp.
       - tauto.
@@ -89,14 +86,15 @@ Section Kripke.
       - destruct q. setoid_rewrite IHphi. split; intros H d; eapply ksat_ext. 2, 4: apply (H d).
         all: intros []; cbn; trivial; unfold funcomp; now erewrite eval_comp.
     Qed.
+
   End Substs.
 
-  Definition kconstraint := forall D, kmodel D -> Prop.
+  (*Definition kconstraint := forall D, kmodel D -> Prop.
   Definition kcon_subs (C C' : kconstraint) := (forall D (M : kmodel D), C' D M -> C D M).
 
-  Definition kstandard D (M : kmodel D) := forall v, k_Bot v -> False.
-  (*Definition kexploding D (M : kmodel D) := forall v rho phi, rho ⊨(v) (falsity --> phi).
-  Definition kexploding' D (M : kmodel D) := forall v rho P t, rho ⊨(v) (⊥ --> Pred P t). 
+  Definition kstandard D (M : kmodel D) := forall v, k_Bot v -> False.*)
+  (*Definition kexploding D (M : kmodel D) := forall v rho phi, rho ⊩(v) (falsity --> phi).
+  Definition kexploding' D (M : kmodel D) := forall v rho P t, rho ⊩(v) (⊥ --> Pred P t). 
   Definition kbottomless D (M : kmodel D) := True.*)
 
   (*Lemma kstandard_explodes :
@@ -107,25 +105,26 @@ Section Kripke.
 
   Context {ff : falsity_flag}.
 
-  Definition kvalid_L (C : kconstraint) A phi :=
-    forall D (M : @kmodel D), C _ M -> forall u rho, (forall psi, psi el A -> ksat u rho psi) -> ksat u rho phi.
+  Definition kvalid_ctx A phi :=
+    forall D (M : kmodel D) u rho, (forall psi, psi el A -> ksat u rho psi) -> ksat u rho phi.
+
+  Definition kvalid phi :=
+    forall D (M : kmodel D) u rho, ksat u rho phi.
+
+  Definition ksatis phi :=
+    exists D (M : kmodel D) u rho, ksat u rho phi.
 
   (*Definition kvalid_T (C : kconstraint) T phi :=
     forall D (M : @kmodel D), C _ M -> forall u rho, (forall psi, psi ∈ T -> ksat u rho psi) -> ksat u rho phi.*)
 
-  Lemma kvalid_L_subs C C' A phi :
-    kcon_subs C' C -> kvalid_L C' A phi -> kvalid_L C A phi.
-  Proof.
-    intros Hsub HC' D M HC % Hsub u rho HA. now apply HC'.
-  Qed.
 End Kripke.
 
-Notation "rho  '⊨(' u ')'  phi" := (ksat u rho phi) (at level 20).
-Notation "rho '⊨(' u , M ')' phi" := (@ksat _ _ M u rho phi) (at level 20).
+Notation "rho  '⊩(' u ')'  phi" := (ksat u rho phi) (at level 20).
+Notation "rho '⊩(' u , M ')' phi" := (@ksat _ _ _ M _ u rho phi) (at level 20).
 (*Notation "A ⊫KE phi" := (kvalid_L kexploding A phi) (at level 20).*)
-Notation "A ⊫KS phi" := (kvalid_L kstandard A phi) (at level 20).
+(*Notation "A ⊫KS phi" := (kvalid A phi) (at level 20).*)
 (*Notation "A ⊫KBL phi" := (kvalid_L kbottomless A phi) (at level 20).*)
-Arguments ksat {_ _} _ _ _ _,  {_} _ _ _ _ _.
+Arguments ksat {_ _ _ _ _} _ _ _, {_ _ _} _ {_} _ _ _.
 
 (** ** Soundness **)
 
@@ -141,85 +140,68 @@ Section KSoundness.
     | [ H : (?A -> ?B), H2 : (?A -> ?B) -> _ |- _] => specialize (H2 H)
     end.
 
-  Lemma ksemantic_explosion D (M : kmodel D) :
-    kexploding' M -> kexploding M.
+  Lemma ksoundness A (phi : form) :
+    A ⊢I phi -> kvalid_ctx A phi.
   Proof.
-    intros H v rho phi.
-    induction phi in rho, v |-*; firstorder.
-  Qed.
-
-  Lemma ksoundness A C (phi : form) :
-    (b = expl -> kcon_subs kexploding C) -> @prv _ intu _ A phi  -> kvalid_L C A phi.
-  Proof.
-    intros Hexp Hprv D M HM. remember intu as s. induction Hprv; subst; cbn; intros u rho HA.
+    intros Hprv D M. remember intu as s. induction Hprv; subst; cbn; intros u rho HA.
     all: repeat (clean_ksoundness + discriminate). all: (eauto || comp; eauto).
-    - intros v Hr Hpi. capply IHHprv. intros ? []; subst; eauto using ksat_mon.
-    - eapply IHHprv1. 3: eapply IHHprv2. all: eauto. reflexivity.
-    - intros d. apply IHHprv. apply switch_map. intros psi Hpsi. rewrite ksat_comp. apply HA, Hpsi.
+    - intros v Hr Hpi. eapply IHHprv. intros ? []; subst; eauto using ksat_mon.
+    - eapply IHHprv1. 3: eapply IHHprv2. all: eauto. apply M.
+    - intros d. apply IHHprv. intros psi [psi' [<- Hp]] % in_map_iff. cbns. rewrite ksat_comp. apply HA, Hp.
     - rewrite ksat_comp. eapply ksat_ext. 2: eapply (IHHprv u rho HA (eval rho t)). 
-      asimpl. now intros [].
-    - apply Hexp in HM. apply (HM u); eauto. apply M.
+      unfold funcomp. now intros [].
+    - now apply IHHprv in HA.
   Qed.
 
-  Lemma strong_ksoundness T C phi :
-    (b = expl -> kcon_subs kexploding C) -> @tprv _ intu _ T phi  -> kvalid_T C T phi.
+  Lemma ksoundness' (phi : form) :
+    [] ⊢I phi -> kvalid phi.
   Proof.
-    intros Hexp (A & HA1 & HA2) D M HM u rho HT. apply (ksoundness Hexp HA2 HM).
-    firstorder.
+    intros H % ksoundness. firstorder.
   Qed.
 
 End KSoundness.
-
-Lemma ksoundness' {Sigma : Signature} A phi :
-  A ⊢IE phi -> A ⊫KS phi.
-Proof.
-  apply ksoundness. intros _. firstorder.
-Qed.
 
 
 
 (** ** Connection to Tarski Semantics *)
 
-Program Instance interp_kripke {domain eta} (I : interp domain eta) : kmodel  eta :=
-  {| nodes := unit ; reachable u v := True |}.
-Next Obligation.
-  all: try abstract tauto.
-  intros. apply emb_refl.
-Defined.
+Section ToTarski.
 
-Lemma kripke_tarski domain eta (b : logic) (I : interp domain eta) rho phi :
-  rho ⊨ phi <-> rho ⊩(tt, interp_kripke I, _) phi.
-Proof.
-  revert rho. induction phi; intros rho.
-  - tauto.
-  - tauto.
-  - tauto.
-  - split; intros H. cbn in *.
-    + intros [] [] H'. apply IHphi2, H,  IHphi1, H'.
-    + intros H'. apply IHphi2, (H tt Logic.I), IHphi1, H'.
-  - split; intros H; cbn in *.
-    + intros [] [] i. apply IHphi, H.
-    + intros i. apply IHphi, (H tt Logic.I).
-Qed.
+  Context {Σ_funcs : funcs_signature}.
+  Context {Σ_preds : preds_signature}.
 
-Definition kvalid b (phi : form b) :=
-  forall domain eta (M : @kmodel domain eta) u rho, rho ⊩(u,M,eta) phi.
+  Program Instance interp_kripke {domain} (I : interp domain) : kmodel domain :=
+    {| nodes := unit ; reachable u v := True |}.
+  Next Obligation.
+    - now apply I in X.
+  Defined.
 
-Definition ksatis b (phi : form b) :=
-  exists domain eta (M : @kmodel domain eta) u rho, ksat eta M u rho phi.
+  Lemma kripke_tarski {ff : falsity_flag} domain (I : interp domain) rho phi :
+    rho ⊨ phi <-> ksat (interp_kripke I) tt rho phi.
+  Proof.
+    revert rho. induction phi; intros rho.
+    - tauto.
+    - tauto.
+    - destruct b0. cbn. rewrite IHphi1, IHphi2. intuition. destruct v. tauto.
+    - destruct q. cbn. split; intros H; cbn in *.
+      + intros i. apply IHphi, H.
+      + intros i. apply IHphi, H.
+  Qed.
 
-Lemma kvalid_valid b (phi : form b) :
-  kvalid phi -> valid phi.
-Proof.
-  intros H domain I eta rho. eapply kripke_tarski, H.
-Qed.
+  Lemma kvalid_valid b (phi : form b) :
+    kvalid phi -> valid phi.
+  Proof.
+    intros H domain I rho. apply kripke_tarski, H.
+  Qed.
 
-Lemma ksatis_satis b (phi : form b) :
-  satis phi -> ksatis phi.
-Proof.
-  intros (domain & eta & I & rho & ?). eapply kripke_tarski in H.
-  now exists domain, eta, (interp_kripke I), tt,  rho.
-Qed.
+  Lemma ksatis_satis b (phi : form b) :
+    satis phi -> ksatis phi.
+  Proof.
+    intros (domain & I & rho & ?). eapply kripke_tarski in H.
+    now exists domain, (interp_kripke I), tt, rho.
+  Qed.
+
+End ToTarski.
 
 
 
